a generally good proof framework (still unsound yet)

core/AssertionLang.v
@@ -1,4 +1,5 @@
 Require Import Coq.ssr.ssrbool.
+Require Import Coq.Strings.String.
 Require Import Poulet4.Typed.
 Require Import Poulet4.Syntax.
 Require Import Poulet4.Semantics.
@@ -10,7 +11,7 @@ Section AssertionLang.
 
 Context {tags_t: Type} {tags_t_inhabitant : Inhabitant tags_t}.
 Notation Val := (@ValueBase tags_t).
-Notation Lval := (@ValueLvalue tags_t).
+Notation SemLval := (@ValueLvalue tags_t).
 
 Notation ident := (P4String.t tags_t).
 Notation path := (list ident).
@@ -21,14 +22,25 @@ Notation Locator := (@Locator tags_t).
 
 Context `{@Target tags_t (@Expression tags_t)}.
 
+Definition Field : Type := string.
+Definition Lval : Type := Locator * list Field.
+
 Definition assertion := list (Lval * Val).
 
 Variable this : path.
 
-Definition sem_eval_read (st : state) (lv : Lval) : option Val :=
+(* Fixpoint sem_eval_read (st : state) (lv : Lval) : option Val :=
   match lv with
   | MkValueLvalue (ValLeftName _ loc) _ =>
       loc_to_val this loc st
+  | MkValueLvalue (ValLeftMember lv member) _ =>
+      match sem_eval_read st lv with
+      | Some (ValBaseStruct fields) =>
+          AList.get fields member
+      | Some (ValBaseHeader fields true) =>
+          AList.get fields member
+      | _ => None
+      end
   | _ => None
   end.
 
@@ -36,11 +48,72 @@ Lemma sem_eval_read_sound : forall st lv v,
   sem_eval_read st lv = Some v ->
   forall v', exec_read this st lv v' ->
     v' = v.
-Admitted.
+Admitted. *)
+
+Definition alist_get {A} (l : P4String.AList tags_t A) (s : string) : option A :=
+  AList.get l (P4String.Build_t _ default s).
+
+Definition extract (v : Val) (f : Field) : option Val :=
+  match v with
+  | ValBaseStruct fields =>
+      alist_get fields f
+  | ValBaseHeader fields true =>
+      alist_get fields f
+  | _ => None
+  end.
+
+Definition extract_option (ov : option Val) (f : Field) : option Val :=
+  match ov with
+  | Some v => extract v f
+  | None => None
+  end.
+
+Definition state_eval_read (st : state) (lv : Lval) : option Val :=
+  let (loc, fl) := lv in
+  fold_left extract_option fl (loc_to_val this loc st).
+
+Definition state_eval_read_alt (st : state) (lv : Lval) : option Val :=
+  let (loc, fl) := lv in
+  let rfl := rev fl in
+  let step (extractor : option Val -> option Val) f ov :=
+    extractor (extract_option ov f) in
+  fold_left step rfl id (loc_to_val this loc st).
+
+Lemma fold_left_fold_right {A B} (f : A -> B -> A) (l : list B) (acc : A) :
+  fold_left f l acc = fold_right (fun x fold_rest acc => fold_rest (f acc x)) id l acc.
+Proof.
+  revert acc.
+  induction l as [ | hd tl]; intros acc.
+  - reflexivity.
+  - change (hd :: tl) with ([hd] ++ tl) at 2.
+    rewrite fold_right_app. simpl. apply IHtl.
+Qed.
+
+Lemma state_eval_read_alt_eq_state_eval_read st lv :
+  state_eval_read_alt st lv = state_eval_read st lv.
+Proof.
+  destruct lv as [loc fl]; simpl.
+  rewrite <- (rev_involutive fl) at 2.
+  rewrite <- fold_left_rev_right with (l := (rev fl)).
+  rewrite fold_left_fold_right.
+  reflexivity.
+Qed.
+
+Definition state_is_valid_field (st : state) (lv : Lval) : bool :=
+  isSome (state_eval_read st lv).
+
+Lemma state_is_valid_field_parent st loc fl1 f :
+  state_is_valid_field st (loc, fl1 ++ [f]) ->
+  state_is_valid_field st (loc, fl1).
+Proof.
+  unfold state_is_valid_field. simpl.
+  rewrite fold_left_app. simpl.
+  destruct (fold_left extract_option fl1 (loc_to_val this loc st)); sfirstorder.
+Qed.
 
 Definition satisfies_unit (st : state) (a_unit : Lval * Val) : Prop :=
   let (lv, v) := a_unit in
-  sem_eval_read st lv = Some v.
+  state_eval_read st lv = Some v.
 
 Definition satisfies (st : state) (a : assertion) : Prop :=
   fold_right and True (map (satisfies_unit st) a).
@@ -54,17 +127,34 @@ Definition loc_no_overlapping (loc1 : Locator) (loc2 : Locator) : bool :=
   | _, _ => false
   end.
 
-Definition lval_no_overlapping (lv1 : Lval) (lv2 : Lval) : bool :=
-  match lv1, lv2 with
-  | MkValueLvalue (ValLeftName _ loc1) _, MkValueLvalue (ValLeftName _ loc2) _ =>
-      loc_no_overlapping loc1 loc2
-  | _, _ => false
+Fixpoint semlval_to_lval (slv : SemLval) : option Lval :=
+  match slv with
+  | MkValueLvalue (ValLeftName _ loc) _ => Some (loc, nil)
+  | MkValueLvalue (ValLeftMember slv member) _ =>
+      let olv := semlval_to_lval slv in
+      option_map (map_snd (cons (P4String.str member))) olv
+  | _ => None
   end.
 
-Fixpoint no_overlapping (lv : Lval) (a : assertion) : bool :=
-  match a with
-  | hd :: tl => lval_no_overlapping lv (fst hd) && no_overlapping lv tl
-  | [] => true
+Definition dummy_type : @P4Type tags_t := TypBool.
+
+Definition lval_to_semlval (lv : Lval) : SemLval :=
+  let (loc, fl) := lv in
+  let acc := MkValueLvalue (ValLeftName (BareName (P4String.Build_t tags_t default "")) loc) dummy_type in
+  let step acc f :=
+      MkValueLvalue (ValLeftMember acc (P4String.Build_t tags_t default f)) dummy_type in
+  fold_left step fl acc.
+
+Lemma state_eval_read_complete : forall st lv v,
+  exec_read this st (lval_to_semlval lv) v ->
+  state_eval_read st lv = Some v.
+Admitted.
+
+Fixpoint field_list_no_overlapping (fl1 fl2 : list Field) : bool :=
+  match fl1, fl2 with
+  | hd1 :: tl1, hd2 :: tl2 =>
+      ~~(String.eqb hd1 hd2) || field_list_no_overlapping tl1 tl2
+  | _, _ => false
   end.
 
 Definition is_instance (loc : Locator) : bool :=
@@ -73,18 +163,29 @@ Definition is_instance (loc : Locator) : bool :=
   | LGlobal _ => false
   end.
 
-Definition is_lval_loc_instance (lv : Lval) : bool :=
+Definition lval_no_overlapping (lv1 : Lval) (lv2 : Lval) : bool :=
+  match lv1, lv2 with
+  | (loc1, fl1), (loc2, fl2) =>
+      is_instance loc1 && is_instance loc2 && (loc_no_overlapping loc1 loc2 || field_list_no_overlapping fl1 fl2)
+  end.
+
+Fixpoint no_overlapping (lv : Lval) (a : assertion) : bool :=
+  match a with
+  | hd :: tl => lval_no_overlapping lv (fst hd) && no_overlapping lv tl
+  | [] => true
+  end.
+
+Definition is_lval_instance (lv : Lval) : bool :=
   match lv with
-  | MkValueLvalue (ValLeftName _ loc) _ =>
+  | (loc, _) =>
       is_instance loc
-  | _ => false
   end.
 
 Fixpoint wellformed (a : assertion) : bool :=
   match a with
   | hd :: tl =>
       let (lv, _) := hd in
-      is_lval_loc_instance lv && no_overlapping lv tl && wellformed tl
+      is_lval_instance lv && no_overlapping lv tl && wellformed tl
   | [] => true
   end.
 
@@ -95,11 +196,16 @@ Definition locator_equivb (loc1 loc2 : Locator) : bool :=
   | _, _ => false
   end.
 
+Definition field_equivb (f1 f2 : Field) : bool :=
+  match f1, f2 with
+  | s1, s2 =>
+      String.eqb s1 s2
+  end.
+
 Definition lval_equivb (lv1 lv2 : Lval) : bool :=
   match lv1, lv2 with
-  | MkValueLvalue (ValLeftName _ loc1) _, MkValueLvalue (ValLeftName _ loc2) _ =>
-      locator_equivb loc1 loc2
-  | _, _ => false
+  | (loc1, fl1), (loc2, fl2) =>
+      locator_equivb loc1 loc2 && list_eqb field_equivb fl1 fl2
   end.
 
 Fixpoint eval_write (a : assertion) (lv : Lval) (v : Val) : assertion :=
@@ -113,14 +219,23 @@ Fixpoint eval_write (a : assertion) (lv : Lval) (v : Val) : assertion :=
   | [] => [(lv, v)]
   end.
 
-Axiom loc_to_val_update_val_by_loc_same : forall st p1 p2 v,
-  path_equivb p1 p2 ->
-  loc_to_val this (LInstance p1) (Semantics.update_val_by_loc this st (LInstance p2) v) = Some v.
+Axiom loc_to_val_update_val_by_loc_same : forall st loc1 loc2 v,
+  locator_equivb loc1 loc2 ->
+  loc_to_val this loc1 (Semantics.update_val_by_loc this st loc2 v) = Some v.
 
-Axiom loc_to_val_update_val_by_loc_different : forall st p1 p2 v,
+Axiom loc_to_val_update_val_by_loc_diff : forall st p1 p2 v,
   ~~ path_equivb p1 p2 ->
   loc_to_val this (LInstance p1) (Semantics.update_val_by_loc this st (LInstance p2) v) =
     loc_to_val this (LInstance p1) st.
+
+Axiom p4string_equivb_refl : forall (s : P4String),
+  P4String.equivb s s.
+
+Axiom p4string_equivb_symm : forall (s1 s2 : P4String),
+  P4String.equivb s1 s2 = P4String.equivb s2 s1.
+
+Axiom p4string_equivb_trans : forall (s1 s2 s3 : P4String),
+  P4String.equivb s1 s2 -> P4String.equivb s2 s3 -> P4String.equivb s1 s3.
 
 Axiom path_equivb_refl : forall (p : path),
   path_equivb p p.
@@ -131,32 +246,316 @@ Axiom path_equivb_symm : forall (p1 p2 : path),
 Axiom path_equivb_trans : forall (p1 p2 p3 : path),
   path_equivb p1 p2 -> path_equivb p2 p3 -> path_equivb p1 p3.
 
+Axiom locator_equivb_refl : forall (loc : Locator),
+  locator_equivb loc loc.
+
+Axiom locator_equivb_symm : forall (loc1 loc2 : Locator),
+  locator_equivb loc1 loc2 = locator_equivb loc2 loc1.
+
+Axiom locator_equivb_trans : forall (loc1 loc2 loc3 : Locator),
+  locator_equivb loc1 loc2 -> locator_equivb loc2 loc3 -> locator_equivb loc1 loc3.
+
 Axiom loc_no_overlapping_symm : forall (loc1 loc2 : Locator),
   loc_no_overlapping loc1 loc2 = loc_no_overlapping loc2 loc1.
 
 Axiom lval_no_overlapping_symm : forall (lv1 lv2 : Lval),
   lval_no_overlapping lv1 lv2 = lval_no_overlapping lv2 lv1.
 
+Axiom lval_equivb_symm : forall (lv1 lv2 : Lval),
+  lval_equivb lv1 lv2 = lval_equivb lv2 lv1.
+
+(* This lemma is not general enough to proof the case in exec_write_no_overlapping_unit,
+  that loc1 = loc2 but the fl1 and fl2 are not overlapping. *)
+
+Lemma lval_to_semlval_snoc loc fl f :
+  lval_to_semlval (loc, fl ++ [f]) =
+    MkValueLvalue (ValLeftMember (lval_to_semlval (loc, fl)) (P4String.Build_t tags_t default f)) dummy_type.
+Proof.
+  simpl. rewrite fold_left_app. reflexivity.
+Qed.
+
+Ltac inv H := inversion H; subst; clear H.
+Ltac pinv P :=
+  lazymatch goal with
+  | H : context [P] |- _ => inv H
+  (* | H : P |- _ => inv H
+  | H : P _ |- _ => inv H
+  | H : P _ _ |- _ => inv H
+  | H : P _ _ _ |- _ => inv H
+  | H : P _ _ _ _ |- _ => inv H
+  | H : P _ _ _ _ _ |- _ => inv H
+  | H : P _ _ _ _ _ _ |- _ => inv H
+  | H : P _ _ _ _ _ _ _ |- _ => inv H
+  | H : P _ _ _ _ _ _ _ _ |- _ => inv H *)
+  end.
+
+Lemma exec_write_1 st lv v st' :
+  exec_write this st (lval_to_semlval lv) v st' ->
+  exists v',
+    st' = update_val_by_loc this st (fst lv) v'.
+Proof.
+  destruct lv as [loc fl]. simpl fst.
+  rewrite <- (rev_involutive fl).
+  generalize dependent v.
+  induction (rev fl) as [ | hd tl]; intros * H_exec_write.
+  - sauto lq: on.
+  - simpl rev in H_exec_write; rewrite lval_to_semlval_snoc in H_exec_write.
+    inv H_exec_write.
+    destruct (IHtl _ ltac:(eassumption)).
+    sfirstorder.
+Qed.
+
+Axiom alist_get_set_same : forall {V} (l l' : P4String.AList tags_t V) (s1 s2 : P4String) v,
+  AList.set l s2 v = Some l' ->
+  P4String.equivb s1 s2 ->
+  AList.get l' s1 = Some v.
+
+Axiom alist_get_set_diff : forall {V} (l l' : P4String.AList tags_t V) (s1 s2 : P4String) v,
+  AList.set l s2 v = Some l' ->
+  ~~P4String.equivb s1 s2 ->
+  AList.get l' s1 = AList.get l s1.
+
+Axiom P4String_equivb_same : forall (tags1 tags2 : tags_t) s1 s2,
+  s1 = s2 ->
+  P4String.equivb (P4String.Build_t _ tags1 s1) (P4String.Build_t _ tags2 s2).
+
+Axiom P4String_equivb_diff : forall (tags1 tags2 : tags_t) s1 s2,
+  s1 <> s2 ->
+  ~~(P4String.equivb (P4String.Build_t _ tags1 s1) (P4String.Build_t _ tags2 s2)).
+
+Hint Resolve alist_get_set_same alist_get_set_diff P4String_equivb_same P4String_equivb_diff : core.
+
+Lemma exec_write_satisfies_unit st lv v st' :
+  state_is_valid_field st lv ->
+  exec_write this st (lval_to_semlval lv) v st' ->
+  satisfies_unit st' (lv, v).
+Proof.
+  intros * H_state_is_valid_field H_exec_write.
+  apply state_eval_read_complete.
+  revert H_state_is_valid_field H_exec_write.
+  (* unfold state_is_valid_field; rewrite <- state_eval_read_alt_eq_state_eval_read; unfold state_eval_read_alt. *)
+  (* rewrite <- lval_to_semlval_alt_eq_lval_to_semlval. *)
+  destruct lv as [loc fl].
+  rewrite <- (rev_involutive fl).
+  generalize dependent v.
+  induction (rev fl) as [ | hd tl]; intros * H_state_is_valid_field H_exec_write.
+  - inv H_exec_write. apply exec_read_name, loc_to_val_update_val_by_loc_same, locator_equivb_refl.
+  - simpl rev in H_exec_write |- *; rewrite lval_to_semlval_snoc in H_exec_write |- *.
+    inv H_exec_write. apply exec_read_by_member.
+    simpl in H_state_is_valid_field.
+    apply state_is_valid_field_parent in H_state_is_valid_field as H_state_is_valid_field'.
+    pinv @update_member.
+    + pinv @write_header_field.
+      eapply exec_read_member_header; only 1 : (apply IHtl; eassumption).
+      rename H5 into H_exec_read.
+      apply (state_eval_read_complete _ (loc, rev tl)) in H_exec_read as H_state_eval_read.
+      destruct is_valid; only 2 : sauto lq: on.
+      eapply read_header_field_intro.
+      eauto.
+    + eapply exec_read_member_struct; only 1 : (apply IHtl; eassumption).
+      eauto.
+    + rename H5 into H_exec_read.
+      apply (state_eval_read_complete _ (loc, rev tl)) in H_exec_read as H_state_eval_read.
+      unfold state_is_valid_field, state_eval_read in H_state_is_valid_field, H_state_eval_read.
+      rewrite fold_left_app in H_state_is_valid_field.
+      rewrite H_state_eval_read in H_state_is_valid_field.
+      discriminate H_state_is_valid_field.
+Qed.
+
+(* Things will be easier if we use the reversed order in exec_write. *)
+
+Lemma satisfies_unit_child st loc fl f fields v :
+  satisfies_unit st ((loc, fl), fields) ->
+  extract_option (Some fields) f = Some v ->
+  satisfies_unit st ((loc, fl ++ [f]), v).
+Proof.
+  simpl. rewrite fold_left_app. hauto lq: on.
+Qed.
+
+(* Proving the following lemma should be enough. For exec_write_no_overlapping_unit,
+  it is easy to remove a last field from either lv1 or lv2, so we can reach the part that
+  only one field is different. *)
+
+Lemma exec_write_2 st loc fl f1 f2 v1 v2 st' :
+  f1 <> f2 ->
+  satisfies_unit st ((loc, fl ++ [f1]), v1) ->
+  exec_write this st (lval_to_semlval (loc, fl ++ [f2])) v2 st' ->
+  satisfies_unit st' ((loc, fl ++ [f1]), v1).
+Proof.
+  intros H_neq H_pre H_exec_write.
+  simpl rev in H_exec_write; rewrite lval_to_semlval_snoc in H_exec_write.
+  inv H_exec_write.
+  eapply satisfies_unit_child with (st := st'). 1 : eapply exec_write_satisfies_unit with (st := st).
+  - eapply state_is_valid_field_parent with (f := f1). unfold satisfies_unit in H_pre.
+    hauto lq: on unfold: isSome, is_true, state_is_valid_field.
+  - eassumption.
+  - apply state_eval_read_complete with (lv := (loc, fl)) in H5 as H_state_eval_read.
+    simpl in H_pre, H_state_eval_read.
+    rewrite fold_left_app, H_state_eval_read in H_pre. simpl in H_pre.
+    clear H_state_eval_read.
+    pinv @update_member.
+    + destruct is_valid; only 2 : sfirstorder.
+      pinv @write_header_field. simpl.
+      rewrite <- H_pre.
+      apply (alist_get_set_diff _ _ _ _ _ H7).
+      srun eauto use: P4String_equivb_diff unfold: default.
+    + rewrite <- H_pre.
+      apply (alist_get_set_diff _ _ _ _ _ H0).
+      srun eauto use: P4String_equivb_diff unfold: default.
+    + inv H_pre.
+Qed.
+
+Lemma exec_write_3 st loc fl1 fl2 v st' :
+  exec_write this st (lval_to_semlval (loc, fl1 ++ fl2)) v st' ->
+  exists v',
+    exec_write this st (lval_to_semlval (loc, fl1)) v' st'.
+Proof.
+  generalize dependent v.
+  rewrite <- (rev_involutive fl2).
+  induction (rev fl2) as [ | hd tl]; intros * H_exec_write.
+  - simpl rev in H_exec_write. rewrite app_nil_r in H_exec_write. sfirstorder.
+  - simpl rev in H_exec_write. rewrite app_assoc in H_exec_write.
+    unfold lval_to_semlval in *. rewrite fold_left_app in H_exec_write.
+    inv H_exec_write; eauto.
+Qed.
+
+(*   state_eval_read st (loc, fl ++ [f2]) = state_eval_read st (loc, fl ++ [f2])
+  exec_write this st (lval_to_semlval lv) v st' ->
+  exists v',
+    st' = update_val_by_loc this st (fst lv) v'.
+Proof.
+  rewrite <- lval_to_semlval_alt_eq_lval_to_semlval.
+  destruct lv as [loc fl]. simpl fst. simpl lval_to_semlval_alt.
+  generalize dependent v.
+  induction (rev fl) as [ | hd tl]; intros * H_exec_write.
+  - sauto lq: on.
+  - inversion H_exec_write; subst.
+    destruct (IHtl _ ltac:(eassumption)).
+    sfirstorder.
+Qed. *)
+
+Lemma exec_write_no_overlapping_unit_case_1 st loc fl f1 f2 v1 v2 st' :
+  let lv1 := (loc, fl ++ [f1]) in
+  let lv2 := (loc, fl ++ [f2]) in
+  lval_no_overlapping lv1 lv2 ->
+  satisfies_unit st (lv1, v1) ->
+  exec_write this st (lval_to_semlval lv2) v2 st' ->
+  satisfies_unit st' (lv1, v1).
+Proof.
+  intros * H_lval_no_overlapping. subst lv1 lv2. apply exec_write_2.
+  unfold lval_no_overlapping in H_lval_no_overlapping.
+  replace (loc_no_overlapping loc loc) with false in H_lval_no_overlapping
+    by (destruct (loc_no_overlapping loc loc) eqn:?;
+      unfold loc_no_overlapping in *; destruct loc; hauto use: path_equivb_refl unfold: is_true, negb).
+  assert (field_list_no_overlapping (fl ++ [f1]) (fl ++ [f2])) as H_field_list_no_overlapping by (hauto b: on).
+  clear H_lval_no_overlapping.
+  induction fl.
+  - simpl in H_field_list_no_overlapping. hauto use: eqb_refl, eqb_neq, Bool.orb_false_l unfold: negb, Field, is_true.
+  - apply IHfl. simpl in H_field_list_no_overlapping. hauto use: eqb_eq unfold: negb, orb, Field, is_true.
+Qed.
+
+(* Lemma exec_write_no_overlapping_unit_case_1_v2 st loc fl f1 f2 v1 v2 st' :
+  let lv1 := (loc, fl ++ [f1]) in
+  let lv2 := (loc, fl ++ [f2]) in
+  f1 <> f2 ->
+  satisfies_unit st (lv1, v1) ->
+  exec_write this st (lval_to_semlval lv2) v2 st' ->
+  satisfies_unit st' (lv1, v1).
+Proof.
+  intros * H_lval_no_overlapping. subst lv1 lv2. apply exec_write_2.
+  (* unfold lval_no_overlapping in H_lval_no_overlapping.
+  replace (loc_no_overlapping loc loc) with false in H_lval_no_overlapping
+    by (destruct (loc_no_overlapping loc loc) eqn:?;
+      unfold loc_no_overlapping in *; destruct loc; hauto use: path_equivb_refl unfold: is_true, negb). *)
+  (* assert (field_list_no_overlapping (fl ++ [f1]) (fl ++ [f2])) as H_field_list_no_overlapping by sfirstorder.
+  clear H_lval_no_overlapping. *)
+  induction fl.
+  - simpl in H_field_list_no_overlapping. hauto use: eqb_refl, eqb_neq, Bool.orb_false_l unfold: negb, Field, is_true.
+  - apply IHfl. simpl in H_field_list_no_overlapping. hauto use: eqb_eq unfold: negb, orb, Field, is_true.
+Qed. *)
+
+Lemma satisfies_unit_child_iff st loc fl f v :
+  satisfies_unit st ((loc, fl ++ [f]), v) <->
+  exists v',
+    satisfies_unit st ((loc, fl), v') /\ extract v' f = Some v.
+Proof.
+  split.
+  - simpl. rewrite fold_left_app. intros H_satisfies_unit.
+    destruct (fold_left extract_option fl (loc_to_val this loc st)) as [v' | ]; only 2 : sfirstorder.
+    exists v'; sfirstorder.
+  - simpl. rewrite fold_left_app. hauto lq: on.
+Qed.
+
+Lemma exec_write_no_overlapping_unit_case_2 st loc fl1 f1 fl2 f2 v1 v2 st' :
+  let lv1 := (loc, fl1 ++ [f1] ++ fl2) in
+  let lv2 := (loc, fl1 ++ [f2]) in
+  f1 <> f2 ->
+  (* lval_no_overlapping lv1 lv2 -> *)
+  satisfies_unit st (lv1, v1) ->
+  exec_write this st (lval_to_semlval lv2) v2 st' ->
+  satisfies_unit st' (lv1, v1).
+Proof.
+  intros * H_lval_no_overlapping H_pre H_exec_write; subst lv1.
+  rewrite <- (rev_involutive fl2) in *.
+  generalize dependent v1.
+  induction (rev fl2) as [ | hd tl]; intros * H_pre.
+  - eapply exec_write_2; eassumption.
+  - simpl rev in *.
+    replace (fl1 ++ [f1] ++ rev tl ++ [hd]) with ((fl1 ++ [f1] ++ rev tl) ++ [hd]) in * by (rewrite <- !app_assoc; reflexivity).
+    rewrite satisfies_unit_child_iff in *.
+    destruct H_pre as [v1' H_pre]; exists v1'.
+    split; only 2 : sfirstorder.
+    apply IHtl; sfirstorder.
+Qed.
+
+Lemma field_list_no_overlapping_spec fl1 fl2 :
+  field_list_no_overlapping fl1 fl2 ->
+  exists fl3 f1 f2 fl4 fl5,
+    f1 <> f2 /\
+    fl1 = fl3 ++ [f1] ++ fl4 /\
+    fl2 = fl3 ++ [f2] ++ fl5.
+Proof.
+Admitted.
+
+(* This axiom is provable if tags_t is a unit type. *)
+Axiom path_equivb_eq : forall (p1 p2 : path), path_equivb p1 p2 -> p1 = p2.
+
+Axiom locator_equivb_eq : forall loc1 loc2, locator_equivb loc1 loc2 -> loc1 = loc2.
+
+Axiom lval_equivb_eq : forall lv1 lv2, lval_equivb lv1 lv2 -> lv1 = lv2.
+
 Lemma exec_write_no_overlapping_unit st lv1 v1 lv2 v2 st' :
   lval_no_overlapping lv1 lv2 ->
   satisfies_unit st (lv1, v1) ->
-  exec_write this st lv2 v2 st' ->
+  exec_write this st (lval_to_semlval lv2) v2 st' ->
   satisfies_unit st' (lv1, v1).
 Proof.
-  intros H_no_overlapping H_pre H_exec.
-  destruct lv1 as [[? loc1 | | |] ?]; only 2-4 : sfirstorder.
-  destruct lv2 as [[? loc2 | | |] ?]; only 2-4 : sfirstorder.
-  inversion H_exec; subst. simpl.
-  destruct loc1; only 1 : sfirstorder.
-  destruct loc2; only 1 : sfirstorder.
-  rewrite loc_to_val_update_val_by_loc_different by sfirstorder.
-  apply H_pre.
+  intros * H_no_overlapping H_pre H_exec_write.
+  destruct lv1 as [loc1 fl1]; destruct lv2 as [loc2 fl2].
+  simpl in H_no_overlapping.
+  destruct loc1 as [ | p1]; only 1 : sfirstorder.
+  destruct loc2 as [ | p2]; only 1 : sfirstorder.
+  destruct (loc_no_overlapping (LInstance p1) (LInstance p2)) eqn:H_loc_no_overlapping.
+  - apply exec_write_3 with (fl1 := []) in H_exec_write.
+    clear v2; destruct H_exec_write as [v2 H_exec_write].
+    inv H_exec_write. simpl.
+    rewrite loc_to_val_update_val_by_loc_diff; only 2 : sfirstorder.
+    apply H_pre.
+  - assert (p1 = p2) by (apply path_equivb_eq; hauto unfold: loc_no_overlapping, negb, is_true); subst p2.
+    
+    assert (field_list_no_overlapping fl1 fl2) as H_field_list_no_overlapping by sfirstorder.
+    apply field_list_no_overlapping_spec in H_field_list_no_overlapping
+      as (fl3 & f1 & f2 & fl4 & fl5 & ? & ? & ?); subst fl1 fl2.
+    rewrite app_assoc in H_exec_write.
+    eapply exec_write_3 in H_exec_write.
+    clear v2; destruct H_exec_write as [v2 H_exec_write].
+    eapply exec_write_no_overlapping_unit_case_2; eassumption.
 Qed.
 
 Lemma exec_write_no_overlapping st a lv v st' :
   no_overlapping lv a ->
   to_shallow_assertion a st ->
-  exec_write this st lv v st' ->
+  exec_write this st (lval_to_semlval lv) v st' ->
   to_shallow_assertion a st'.
 Proof.
   intros H_no_overlapping H_pre H_exec.
@@ -164,9 +563,9 @@ Proof.
   - sfirstorder.
   - split.
     + destruct hd as [a_lv a_v].
-      eapply (exec_write_no_overlapping_unit st _ _ lv v).
+      eapply (exec_write_no_overlapping_unit).
       * rewrite lval_no_overlapping_symm. hauto b: on.
-      * sfirstorder.
+      * apply H_pre.
       * sfirstorder.
     + apply IHtl.
       * hauto b: on.
@@ -174,26 +573,58 @@ Proof.
 Qed.
 
 Lemma exec_write_same st lv v st' :
-  is_lval_loc_instance lv ->
-  exec_write this st lv v st' ->
+  state_is_valid_field st lv ->
+  exec_write this st (lval_to_semlval lv) v st' ->
   satisfies_unit st' (lv, v).
 Proof.
-  intros H_is_lval_loc_instance H_exec_write.
-  simpl. destruct lv as [[? loc | | |] ?]; only 2-4 : sfirstorder.
-  inversion H_exec_write; subst.
-  simpl. destruct loc; only 1 : sfirstorder.
-  apply loc_to_val_update_val_by_loc_same.
-  apply path_equivb_refl.
+  apply exec_write_satisfies_unit.
 Qed.
 
+Fixpoint eval_read (a : assertion) (lv : Lval) : option Val :=
+  match a with
+  | (hd_lv, hd_v) :: tl =>
+      if lval_equivb hd_lv lv then Some hd_v else eval_read tl lv
+  | [] => None
+  end.
+
+Definition isNil {A} (l : list A) :=
+  match l with
+  | nil => true
+  | _ => false
+  end.
+
+Definition is_valid_field (a : assertion) (lv : Lval) : bool :=
+  let (loc, fl) := lv in
+  isNil fl || isSome (eval_read a lv).
+
+Definition is_valid_field_sound st a lv :
+  to_shallow_assertion a st ->
+  is_valid_field a lv ->
+  state_is_valid_field st lv.
+Admitted.
+
 Lemma eval_write_add st a lv v st':
-  is_lval_loc_instance lv ->
+  is_valid_field a lv ->
   no_overlapping lv a ->
   to_shallow_assertion a st ->
-  exec_write this st lv v st' ->
+  exec_write this st (lval_to_semlval lv) v st' ->
   to_shallow_assertion ((lv, v) :: a) st'.
 Proof.
-  intros H_is_lval_loc_instance H_no_overlapping H_pre H_exec_write.
+  intros H_is_valid_field H_no_overlapping H_pre H_exec_write.
+  split.
+  - eapply exec_write_same; only 2 : eassumption.
+    eapply is_valid_field_sound; eassumption.
+  - apply (exec_write_no_overlapping st _ lv v); sfirstorder.
+Qed.
+
+Lemma eval_write_add' st a lv v st':
+  state_is_valid_field st lv ->
+  no_overlapping lv a ->
+  to_shallow_assertion a st ->
+  exec_write this st (lval_to_semlval lv) v st' ->
+  to_shallow_assertion ((lv, v) :: a) st'.
+Proof.
+  intros H_is_valid_field H_no_overlapping H_pre H_exec_write.
   split.
   - eapply exec_write_same; eassumption.
   - apply (exec_write_no_overlapping st _ lv v); sfirstorder.
@@ -211,37 +642,31 @@ Fixpoint no_nequiv_overlapping (lv : Lval) (a : assertion) : bool :=
 
 Lemma eval_write_sound : forall st a lv v st',
   wellformed a ->
-  is_lval_loc_instance lv ->
+  is_valid_field a lv ->
+  is_lval_instance lv ->
   no_nequiv_overlapping lv a ->
   to_shallow_assertion a st ->
-  exec_write this st lv v st' ->
+  exec_write this st (lval_to_semlval lv) v st' ->
   to_shallow_assertion (eval_write a lv v) st'.
 Proof.
-  intros * H_wellformed H_is_lval_loc_instance H_no_nequiv_overlapping H_pre H_exec_write.
+  intros * H_wellformed H_is_valid_field H_is_lval_instance H_no_nequiv_overlapping H_pre H_exec_write.
   induction a as [ | hd tl]; intros.
   - eapply eval_write_add; eassumption.
   - destruct hd as [hd_lv hd_v].
     simpl in H_no_nequiv_overlapping |- *. destruct (lval_equivb lv hd_lv) eqn:H_lval_equivb.
-    + eapply eval_write_add with (st := st); sfirstorder.
+    + eapply eval_write_add' with (st := st); only 2-4 : sfirstorder.
+      eapply is_valid_field_sound; eassumption.
     + split.
       * refine (exec_write_no_overlapping_unit _ _ _ _ _ _ _ _ H_exec_write); only 2 : sfirstorder.
-        hauto use: lval_no_overlapping_symm unfold: is_true, andb.
-      * apply IHtl; only 3 : sfirstorder; hauto b: on.
+        hauto brefl: on use: lval_no_overlapping_symm unfold: andb, is_true.
+      * apply IHtl; only 4 : sfirstorder; only 1, 3: hauto b: on.
+        destruct lv as [loc fl].
+        simpl in H_is_valid_field.
+        replace (lval_equivb hd_lv (loc, fl)) with (false) in H_is_valid_field by (rewrite lval_equivb_symm; sfirstorder).
+        sfirstorder.
 Qed.
 
-Fixpoint eval_read (a : assertion) (lv : Lval) : option Val :=
-  match a with
-  | (hd_lv, hd_v) :: tl =>
-      if lval_equivb hd_lv lv then Some hd_v else eval_read tl lv
-  | [] => None
-  end.
-
-(* This axiom is provable if tags_t is a unit type. *)
-Axiom locator_equivb_eq : forall loc1 loc2, locator_equivb loc1 loc2 -> loc1 = loc2.
-
-Axiom lval_equivb_eq : forall lv1 lv2, lval_equivb lv1 lv2 -> lv1 = lv2.
-
-Lemma eval_read_sound : forall st a lv v,
+(* Lemma eval_read_sound : forall st a lv v,
   to_shallow_assertion a st ->
   eval_read a lv = Some v ->
   sem_eval_read st lv = Some v.
@@ -255,7 +680,7 @@ Proof.
     + erewrite <- (lval_equivb_eq _ lv) by (apply H_lval_equivb).
       sfirstorder.
     + apply IHtl; sfirstorder.
-Qed.
+Qed. *)
 
 End AssertionLang.
 
